Split up some of Machine into AbstractAnalysis and Semantics and added operational semantics

Machine.v
@@ -1,5 +1,6 @@
 (*Require Import Coq.FSets.FMaps.*)
 Require Import Coq.Lists.List.
+Require Import Bits.
 (*Require Import Coq.Vectors.Vector.*)
 (*Require Import SFI.Machine.Bits.*)
 (*Require Import bbv.Word.*)
@@ -28,6 +29,34 @@ Inductive register : Set :=
 | r14
 | r15.
 
+Inductive value : Set :=
+| A_Reg : register -> value
+| A_Const : int64 -> value
+| A_MultPlus : int64 -> value -> value -> value.
+
+Fixpoint update {A} (l : list A) (i : nat) (v : A) : list A :=
+match l, i with
+| nil , _ => l
+| h :: t, 0 => v :: t
+| h :: t, S i' => update t i' v
+end.
+
+Inductive instr_class := 
+| Heap_Read : register -> register -> register -> instr_class
+| Heap_Write : register -> register -> register -> instr_class
+| Heap_Check : register -> instr_class
+(*| Branch : flags_ty -> instr_class*)
+| CF_Check : register -> instr_class
+| Reg_Move : register -> register -> instr_class
+| Reg_Write : register -> value -> instr_class
+| Stack_Expand : nat -> instr_class
+| Stack_Contract : nat -> instr_class
+| Stack_Read : register -> nat -> instr_class
+| Stack_Write : nat -> register -> instr_class
+| Indirect_Call : register -> instr_class
+| Direct_Call : instr_class
+| Ret : instr_class.
+
 Definition register_eq_dec : forall (x y:register), {x=y} + {x<>y}.
   intros ; decide equality.
 Defined.
@@ -39,13 +68,6 @@ Inductive flag : Set :=
 | pf
 | cf.
 
-Inductive info : Set :=
-| unbounded
-| mem_bounded
-| cf_bounded
-| heap_base.
-
-
 Definition fmap (A B:Type) := 
   A -> B.
 
@@ -54,268 +76,4 @@ Definition set {A} (eq_dec:forall (x y:A),{x=y}+{x<>y}) {B} (f:fmap A B) (x:A) (
 
 Definition get {A} {B} (f:fmap A B) (x:A) : B := 
   f x.
-
-Definition registers_ty := fmap register info.
-
-Definition frame_ty := list info.
-
-Definition stack_ty := list frame_ty.
-
-(* Definition heap_ty := list info.*)
-
-(* Definition flags_ty := fmap flag state. *)
-
-Record state := {
-  regs : registers_ty;
-(*  flags : flags_ty; *)
-  frame : frame_ty;
-  stack : stack_ty;
-(*  heap : heap_ty; *)
-}.
-
-Definition empty_state :=
-{| regs := fun r => if register_eq_dec r rdi then heap_base else unbounded;
-   frame := nil;
-   stack := nil;
-(*   heap := nil *)|}.
-
-(*
-Inductive value : Set :=
-| A_Reg : register -> value
-| A_Const : word64 -> value
-| A_MultPlus : word64 -> value -> value -> value.
-*)
-
-(*
-Fixpoint value_to_word64 (s : machine) (v :value) : word64 :=
-match v with
-| A_Reg r => (regs s) r
-| A_Const c => c
-| A_MultPlus m v1 v2 => wmult m (wplus (value_to_word64 s v1) (value_to_word64 s v2))
-end.
-*)
-
-(*
-Definition read_register (s : machine) (r : register) : word64 :=
-  get register word64 s.(regs) r.
-*)
-
-(*
-Definition write_register (s : machine) (r : register) (v : word64) : machine :=
-{| regs := set register register_eq_dec word64 s.(regs) r v;
-   flags := s.(flags);
-   stack := s.(stack);
-   heap := s.(heap) |}.
-*)
-
-(*
-Definition set_flags (s : machine) (f : flags_ty) : machine :=
-{| regs := s.(regs);
-   flags := f;
-   stack := s.(stack);
-   heap := s.(heap) |}. 
-*)
-
-Definition expand_stack (s : state) (i : nat) : state :=
-{| regs := s.(regs);
-(*   flags := s.(flags); *)
-   frame := s.(frame) ++ (repeat unbounded i);
-   stack := s.(stack);
-(*   heap := s.(heap) *)|}.
-
-Fixpoint contract_stack (s : state) (i : nat) : state :=
-match i with
-| 0 => s
-| S n =>
-contract_stack {| regs := s.(regs);
-(*   flags := s.(flags); *)
-   frame := removelast s.(frame);
-   stack := s.(stack);
-(*   heap := s.(heap) *) |} n
-end.
-
-(*
-Definition read_stack_word (s : machine) (i : nat) : word8 :=
-match nth_error s.(stack) i with
-| Some v => v
-| None => wzero8 (* we might want to do something else here *)
-end.
-*)
-
-(*
-Program Fixpoint read_stack (s : machine) (i : nat) (sz : nat) : word (8 * sz):=
-match sz with
-| 0 => WO
-| S sz' => combine (read_stack_word s i) (read_stack s (i+1) (sz'))
-end.
-Next Obligation. rewrite <- plus_n_O. repeat (rewrite <- plus_n_Sm). reflexivity.
-Qed.
-*)
-
-(*
-Definition read_heap_word (s : machine) (key :  word64) : word8 :=
- s.(heap) key.
-*)
-
-(*
-Program Fixpoint read_heap (s : machine) (key : word64) (sz : nat) : word (8 * sz):=
-match sz with
-| 0 => WO
-| S sz' => combine (read_heap_word s key) (read_heap s (wplus key (wone 64)) (sz'))
-end.
-Next Obligation. rewrite <- plus_n_O. repeat (rewrite <- plus_n_Sm). reflexivity.
-Qed.
-*)
-
-Definition get_register_info (s : state) (r : register) : info :=
-  get s.(regs) r.
-
-Definition set_register_info (s : state) (r : register) (i : info) : state :=
-{| regs := set register_eq_dec s.(regs) r i;
-   frame := s.(frame);
-   stack := s.(stack);
-(*   heap := s.(heap) *) |}.
-
-Definition get_stack_info (s : state) (index : nat) : info :=
-nth index s.(frame) unbounded.
-
-Definition pop_frame (s : state) : state :=
-{| regs := s.(regs);
-   frame := last s.(stack) nil;
-   stack := tail s.(stack);
-(*   heap := s.(heap) *) |}.
-
-Definition push_frame (s : state) : state :=
-{| regs := s.(regs);
-   frame := nil;
-   stack := s.(frame) :: s.(stack);
-(*   heap := s.(heap) *) |}.
-
-Fixpoint update {A} (l : list A) (i : nat) (v : A) : list A :=
-match l, i with
-| nil , _ => l
-| h :: t, 0 => v :: t
-| h :: t, S i' => update t i' v
-end.
-
-(* this needs to be updated *)
-Definition set_stack_info (s : state) (index : nat) (i : info) : state :=
-{| regs := s.(regs);
-   frame := update s.(frame) index i;
-   stack := s.(stack);
- (*  heap := s.(heap) *) |}.
-
-Definition empty {A} (l : list A) :=
-  l = nil.
-
-Inductive instr_class := 
-| Heap_Read : register -> register -> register -> instr_class
-| Heap_Write : register -> register -> register -> instr_class
-| Heap_Check : register -> instr_class
-(*| Branch : flags_ty -> instr_class*)
-| CF_Check : register -> instr_class
-| Reg_Move : register -> register -> instr_class
-| Reg_Write : register (*-> register *)-> instr_class
-| Stack_Expand : nat -> instr_class
-| Stack_Contract : nat -> instr_class
-| Stack_Read : register -> nat -> instr_class
-| Stack_Write : nat -> register -> instr_class
-| Indirect_Call : register -> instr_class
-| Direct_Call : instr_class
-| Ret : instr_class.
-
-Reserved Notation " st '|-' i '⟶' st' "
-                  (at level 40, st' at level 39).
-Inductive instr_class_step : instr_class -> state -> state -> Prop := 
-| I_Heap_Read: forall st r_base r_src r_dst,
-    (* r_base <> r_src -> *) (* not sure if we need this to make the proofs easier *)
-    get_register_info st r_base = heap_base ->
-    get_register_info st r_src = mem_bounded ->
-    st |- (Heap_Read r_dst r_src r_base) ⟶ (set_register_info st r_dst unbounded) 
-| I_Heap_Write: forall st r_base r_src r_dst,
-    (* r_base <> r_src -> *) (* not sure if we need this to make the proofs easier *)
-    get_register_info st r_base = heap_base ->
-    get_register_info st r_src = mem_bounded -> 
-    st |- (Heap_Write r_dst r_src r_base) ⟶ st
-| I_Heap_Check: forall st r_src,
-    st |- (Heap_Check r_src) ⟶ (set_register_info st r_src mem_bounded)
-| I_CF_Check: forall st r_src,
-    st |- (CF_Check r_src) ⟶ (set_register_info st r_src cf_bounded)
-| I_Reg_Move: forall st r_src r_dst,
-    st |- (Reg_Move r_dst r_src) ⟶ (set_register_info st r_dst (get_register_info st r_src))
-| I_Reg_Write: forall st r_dst,
-    st |- (Reg_Write r_dst) ⟶ (set_register_info st r_dst unbounded)
-| I_Stack_Expand: forall st i,
-    st |- (Stack_Expand i) ⟶ (expand_stack st i)
-| I_Stack_Contract: forall st i,
-    st |- (Stack_Contract i) ⟶ (contract_stack st i)
-| I_Stack_Read: forall st i r_dst,
-    i < (length st.(frame)) ->
-    st |- (Stack_Read r_dst i) ⟶ (set_register_info st r_dst (get_stack_info st i))
-| I_Stack_Write: forall st i r_src,
-    i < (length st.(frame)) ->
-    st |- (Stack_Write i r_src) ⟶ (set_stack_info st i (get_register_info st r_src))
-| I_Indirect_Call: forall st reg,
-    get_register_info st reg = cf_bounded ->
-    get_register_info st rdi = heap_base ->
-    st |- (Indirect_Call reg) ⟶ (push_frame st)
-| I_Direct_Call: forall st,
-    get_register_info st rdi = heap_base ->
-    st |- (Direct_Call) ⟶ (push_frame st)
-| I_Ret: forall st,
-    empty st.(frame) ->
-    st |- (Ret) ⟶ (pop_frame st)
-  where " st '|-' i '⟶' st' " := (instr_class_step i st st').
-
-Reserved Notation " st '|-' is '\longrightarrow*' st' "
-                  (at level 40, st' at level 39).
-Inductive instr_class_multi : instr_class -> state -> state -> Prop := .
-
-Definition basic_block := list instr_class.
-
-Record cfg_ty := {
-  nodes : list basic_block;
-  edges : list (basic_block * basic_block)
-}.
-
-Lemma register_get_after_set_eq : forall (regs : registers_ty) reg v,
-    get (set register_eq_dec regs reg v) reg = v.
-Proof.
-  intros regs reg v. unfold get. unfold set. destruct (register_eq_dec reg reg).
-  - reflexivity.
-  - exfalso. apply n. reflexivity.
-Qed.
-
-Lemma register_get_after_set_neq : forall (regs : registers_ty) reg1 reg2 v,
-    reg1 <> reg2 ->
-    get (set register_eq_dec regs reg2 v) reg1 = get regs reg1.
-Proof.
-  intros regs reg1 reg2 v Heq. unfold get. unfold set. destruct (register_eq_dec reg2 reg1).
-  - exfalso. apply Heq. auto.
-  - reflexivity.
-Qed.
-
-Definition safe_stack_read (st : state) (r_base : register) (r_src : register) (r_dst : register) : Prop :=
-  r_base <> r_src /\ get_register_info st r_base = heap_base /\ get_register_info st r_src = mem_bounded.
-
-Lemma read_after_check_is_safe: forall r_base r_src r_dst st, exists st' st'',
-  r_base <> r_src ->
-  get_register_info st r_base = heap_base ->
-  st |- (Heap_Check r_src) ⟶ st' /\ st' |- (Heap_Read r_dst r_src r_base) ⟶ st''.
-Proof.
-  intros r_base r_src r_dst st. 
-  eexists. eexists. intros Hneq Hbase.
-  split.
-  - apply I_Heap_Check.
-  - apply I_Heap_Read.
-    + unfold get_register_info in *. unfold set_register_info. simpl. rewrite register_get_after_set_neq; auto.
-    + unfold get_register_info in *. unfold set_register_info. simpl. rewrite register_get_after_set_eq; auto.
-Qed.
-
-Theorem sfi_property: forall (cfg : cfg_ty) exists st,
-  (* local properties -> *)
- empty |- cfg --> st.
-
-Definition terminates (instrs : list instr_class) : Prop :=
-  exists st, fold_left instr_class_step empty_state instrs = st.
 
