AbstractAnalysis.v
@@ -1,0 +1,229 @@
+Require Import Machine.
+
+Inductive info : Set :=
+| unbounded
+| mem_bounded
+| cf_bounded
+| heap_base.
+
+Definition abs_registers_ty := fmap register info.
+
+Definition abs_stack_ty := list info.
+
+(* Definition heap_ty := list info.*)
+
+(* Definition flags_ty := fmap flag state. *)
+
+Record abs_state := {
+  regs : registers_ty;
+(*  flags : flags_ty; *)
+  stack : stack_ty;
+(*  heap : heap_ty; *)
+}.
+
+Definition abs_empty_state :=
+{| regs := fun r => if register_eq_dec r rdi then heap_base else unbounded;
+   stack := nil;
+(*   heap := nil *)|}.
+
+(*
+Inductive value : Set :=
+| A_Reg : register -> value
+| A_Const : word64 -> value
+| A_MultPlus : word64 -> value -> value -> value.
+*)
+
+(*
+Fixpoint value_to_word64 (s : machine) (v :value) : word64 :=
+match v with
+| A_Reg r => (regs s) r
+| A_Const c => c
+| A_MultPlus m v1 v2 => wmult m (wplus (value_to_word64 s v1) (value_to_word64 s v2))
+end.
+*)
+
+(*
+Definition read_register (s : machine) (r : register) : word64 :=
+  get register word64 s.(regs) r.
+*)
+
+(*
+Definition write_register (s : machine) (r : register) (v : word64) : machine :=
+{| regs := set register register_eq_dec word64 s.(regs) r v;
+   flags := s.(flags);
+   stack := s.(stack);
+   heap := s.(heap) |}.
+*)
+
+(*
+Definition set_flags (s : machine) (f : flags_ty) : machine :=
+{| regs := s.(regs);
+   flags := f;
+   stack := s.(stack);
+   heap := s.(heap) |}. 
+*)
+
+Definition expand_stack (s : state) (i : nat) : state :=
+{| regs := s.(regs);
+(*   flags := s.(flags); *)
+   stack := s.(stack) ++ (repeat unbounded i);
+(*   heap := s.(heap) *)|}.
+
+Fixpoint contract_stack (s : state) (i : nat) : state :=
+match i with
+| 0 => s
+| S n =>
+contract_stack {| regs := s.(regs);
+(*   flags := s.(flags); *)
+   stack := removelast s.(stack);
+(*   heap := s.(heap) *) |} n
+end.
+
+(*
+Definition read_stack_word (s : machine) (i : nat) : word8 :=
+match nth_error s.(stack) i with
+| Some v => v
+| None => wzero8 (* we might want to do something else here *)
+end.
+*)
+
+(*
+Program Fixpoint read_stack (s : machine) (i : nat) (sz : nat) : word (8 * sz):=
+match sz with
+| 0 => WO
+| S sz' => combine (read_stack_word s i) (read_stack s (i+1) (sz'))
+end.
+Next Obligation. rewrite <- plus_n_O. repeat (rewrite <- plus_n_Sm). reflexivity.
+Qed.
+*)
+
+(*
+Definition read_heap_word (s : machine) (key :  word64) : word8 :=
+ s.(heap) key.
+*)
+
+(*
+Program Fixpoint read_heap (s : machine) (key : word64) (sz : nat) : word (8 * sz):=
+match sz with
+| 0 => WO
+| S sz' => combine (read_heap_word s key) (read_heap s (wplus key (wone 64)) (sz'))
+end.
+Next Obligation. rewrite <- plus_n_O. repeat (rewrite <- plus_n_Sm). reflexivity.
+Qed.
+*)
+
+Definition get_register_info (s : state) (r : register) : info :=
+  get s.(regs) r.
+
+Definition set_register_info (s : state) (r : register) (i : info) : state :=
+{| regs := set register_eq_dec s.(regs) r i;
+   stack := s.(stack);
+(*   heap := s.(heap) *) |}.
+
+Definition get_stack_info (s : state) (index : nat) : info :=
+nth index s.(stack) unbounded.
+
+(* this needs to be updated *)
+Definition set_stack_info (s : state) (index : nat) (i : info) : state :=
+{| regs := s.(regs);
+   stack := update s.(stack) index i;
+ (*  heap := s.(heap) *) |}.
+
+Definition empty {A} (l : list A) :=
+  l = nil.
+
+Reserved Notation " st '|-' i '⟶' st' "
+                  (at level 40, st' at level 39).
+Inductive instr_class_flow_function : instr_class -> state -> state -> Prop := 
+| I_Heap_Read: forall st r_base r_src r_dst,
+    (* r_base <> r_src -> *) (* not sure if we need this to make the proofs easier *)
+    get_register_info st r_base = heap_base ->
+    get_register_info st r_src = mem_bounded ->
+    st |- (Heap_Read r_dst r_src r_base) ⟶ (set_register_info st r_dst unbounded) 
+| I_Heap_Write: forall st r_base r_src r_dst,
+    (* r_base <> r_src -> *) (* not sure if we need this to make the proofs easier *)
+    get_register_info st r_base = heap_base ->
+    get_register_info st r_src = mem_bounded -> 
+    st |- (Heap_Write r_dst r_src r_base) ⟶ st
+| I_Heap_Check: forall st r_src,
+    st |- (Heap_Check r_src) ⟶ (set_register_info st r_src mem_bounded)
+| I_CF_Check: forall st r_src,
+    st |- (CF_Check r_src) ⟶ (set_register_info st r_src cf_bounded)
+| I_Reg_Move: forall st r_src r_dst,
+    st |- (Reg_Move r_dst r_src) ⟶ (set_register_info st r_dst (get_register_info st r_src))
+| I_Reg_Write: forall st r_dst,
+    st |- (Reg_Write r_dst) ⟶ (set_register_info st r_dst unbounded)
+| I_Stack_Expand: forall st i,
+    st |- (Stack_Expand i) ⟶ (expand_stack st i)
+| I_Stack_Contract: forall st i,
+    st |- (Stack_Contract i) ⟶ (contract_stack st i)
+| I_Stack_Read: forall st i r_dst,
+    i < (length st.(stack)) ->
+    st |- (Stack_Read r_dst i) ⟶ (set_register_info st r_dst (get_stack_info st i))
+| I_Stack_Write: forall st i r_src,
+    i < (length st.(stack)) ->
+    st |- (Stack_Write i r_src) ⟶ (set_stack_info st i (get_register_info st r_src))
+| I_Indirect_Call: forall st reg,
+    get_register_info st reg = cf_bounded ->
+    get_register_info st rdi = heap_base ->
+    st |- (Indirect_Call reg) ⟶  st
+| I_Direct_Call: forall st,
+    get_register_info st rdi = heap_base ->
+    st |- (Direct_Call) ⟶  st
+| I_Ret: forall st,
+    empty st.(stack) ->
+    st |- (Ret) ⟶  st
+  where " st '|-' i '⟶' st' " := (instr_class_flow_function i st st').
+
+Reserved Notation " st '|-' is '\longrightarrow*' st' "
+                  (at level 40, st' at level 39).
+Inductive instr_class_multi : instr_class -> state -> state -> Prop := .
+
+Definition basic_block := list instr_class.
+
+Record cfg_ty := {
+  nodes : list basic_block;
+  edges : list (basic_block * basic_block)
+}.
+
+Lemma register_get_after_set_eq : forall (regs : registers_ty) reg v,
+    get (set register_eq_dec regs reg v) reg = v.
+Proof.
+  intros regs reg v. unfold get. unfold set. destruct (register_eq_dec reg reg).
+  - reflexivity.
+  - exfalso. apply n. reflexivity.
+Qed.
+
+Lemma register_get_after_set_neq : forall (regs : registers_ty) reg1 reg2 v,
+    reg1 <> reg2 ->
+    get (set register_eq_dec regs reg2 v) reg1 = get regs reg1.
+Proof.
+  intros regs reg1 reg2 v Heq. unfold get. unfold set. destruct (register_eq_dec reg2 reg1).
+  - exfalso. apply Heq. auto.
+  - reflexivity.
+Qed.
+
+Definition safe_stack_read (st : state) (r_base : register) (r_src : register) (r_dst : register) : Prop :=
+  r_base <> r_src /\ get_register_info st r_base = heap_base /\ get_register_info st r_src = mem_bounded.
+
+Lemma read_after_check_is_safe: forall r_base r_src r_dst st, exists st' st'',
+  r_base <> r_src ->
+  get_register_info st r_base = heap_base ->
+  st |- (Heap_Check r_src) ⟶ st' /\ st' |- (Heap_Read r_dst r_src r_base) ⟶ st''.
+Proof.
+  intros r_base r_src r_dst st. 
+  eexists. eexists. intros Hneq Hbase.
+  split.
+  - apply I_Heap_Check.
+  - apply I_Heap_Read.
+    + unfold get_register_info in *. unfold set_register_info. simpl. rewrite register_get_after_set_neq; auto.
+    + unfold get_register_info in *. unfold set_register_info. simpl. rewrite register_get_after_set_eq; auto.
+Qed.
+
+Theorem sfi_property: forall (cfg : cfg_ty) exists st,
+  (* local properties -> *)
+ empty |- cfg --> st.
+
+Definition terminates (instrs : list instr_class) : Prop :=
+  exists st, fold_left instr_class_flow_function empty_state instrs = st.
+
