Semantics.v
@@ -1,0 +1,101 @@
+Require Import Coq.Lists.List.
+Require Import BinInt.
+Require Import Machine.
+Require Import Bits.
+
+(*TODO: figure out if we need uints vs ints*)
+Definition registers_ty := fmap register int64.
+
+Definition stack_ty := list int64.
+
+Definition heap_ty := fmap int64 int64.
+
+Definition flags_ty := fmap flag int1.
+
+Record state := {
+  regs : registers_ty;
+  flags : flags_ty;
+  stack : stack_ty;
+  heap : heap_ty;
+}.
+
+Fixpoint value_to_int64 (s : state) (v :value) : int64 :=
+match v with
+| A_Reg r => (regs s) r
+| A_Const c => c
+| A_MultPlus m v1 v2 => Word.mul m (Word.add (value_to_int64 s v1) (value_to_int64 s v2))
+end.
+
+Definition get_register (s : state) (r : register) : int64 :=
+  get s.(regs) r.
+
+Definition set_register (s : state) (r : register) (v : int64) : state :=
+{| regs := set register_eq_dec s.(regs) r v;
+   flags := s.(flags);
+   stack := s.(stack);
+   heap := s.(heap) |}.
+
+Definition set_flags (s : state) (f : flags_ty) : state :=
+{| regs := s.(regs);
+   flags := f;
+   stack := s.(stack);
+   heap := s.(heap) |}. 
+
+Definition expand_stack (s : state) (i : nat) : state :=
+{| regs := s.(regs);
+   flags := s.(flags);
+   stack := s.(stack) ++ (repeat Word.zero i);
+   heap := s.(heap) |}.
+
+Fixpoint contract_stack (s : state) (i : nat) : state :=
+match i with
+| 0 => s
+| S n =>
+contract_stack {| regs := s.(regs);
+   flags := s.(flags);
+   stack := removelast s.(stack);
+   heap := s.(heap) |} n
+end.
+
+Definition read_stack (s : state) (i : nat) : int64 :=
+nth_default Word.zero s.(stack) i.
+
+Definition write_stack (s : state) (i : nat) (val : int64) : state :=
+{| regs := s.(regs);
+   flags := s.(flags);
+   stack := update s.(stack) i val;
+   heap := s.(heap) |}.
+
+Definition int64_eq_dec : forall x y : int64, { eq x y } + { ~ eq x y }.
+Proof.
+	intros. case_eq (Word.eq x y); intros.
+		- left. inversion H. admit.  (*unfold eq; int_to_Z_tac. omega.*)
+		- right. unfold Word.eq in H. admit. (*unfold eq; int_to_Z_tac. omega.*)
+Admitted.
+
+Definition read_heap (s : state) (i : int64) : int64 :=
+s.(heap) i.
+
+Definition write_heap (s : state) (i : int64) (v : int64) : state :=
+{| regs := s.(regs);
+	 flags := s.(flags);
+	 stack := s.(stack);
+	 heap := set int64_eq_dec s.(heap) i v |}.
+
+Definition run_instr (inst : instr_class) (s : state) : state := 
+  match inst with 
+| Heap_Read r_dst r_src r_base => set_register s r_dst (read_heap s (Word.add (get_register s r_src) (get_register s r_base)))
+| Heap_Write r_dst r_val r_base => write_heap s (Word.add (get_register s r_dst) (get_register s r_base)) (get_register s r_val)
+| Heap_Check r => set_register s r (Word.modu (get_register s r) (Word.shl (Word.repr 2) (Word.repr 32)))
+| CF_Check r => s (*TODO: Figure out wtf to do.*)
+| Reg_Write r v => set_register s r (value_to_int64 s v)
+| Reg_Move r_dst r_src => set_register s r_dst (get_register s r_src)
+| Stack_Expand i => expand_stack s i
+| Stack_Contract i => contract_stack s i
+| Stack_Read r i => set_register s r (read_stack s i)
+| Stack_Write i r => write_stack s i (get_register s r)
+(*TODO: Make sure calls are right*)
+| Indirect_Call r => s
+| Direct_Call => s
+| Ret => s
+end.
